Typing.v
@@ -3,107 +3,207 @@
 (* (C) 2020 Nandor Licker. All rights reserved. *)
 
 Require Import Coq.Lists.List.
+Require Import Coq.ZArith.ZArith.
 
 Require Import LLIR.State.
 Require Import LLIR.LLIR.
 Require Import LLIR.Maps.
+Require Import LLIR.Values.
 
 
 Definition type_env := PTrie.t ty.
 
-Definition ptr_ty := I64.
 
 
+(* Interface containing all target-specific information. *)
+Module Type ArchTy.
+  Parameter ptr_ty: ty.
+End ArchTy.
 
-Definition get_inst_def (i: inst): option (ty * reg) :=
-  match i with
-  | LLInvoke dst _ _ _ _ => dst
+(* X86-specific typing. *)
+Module X86_ArchTy <: ArchTy.
+  Definition ptr_ty := TInt I64.
+End X86_ArchTy.
 
-  | LLArg dst _ _ => Some dst
-  | LLInt8 dst _ _ => Some (I8, dst)
-  | LLInt16 _ dst _ => Some (I16, dst)
-  | LLInt32 _ dst _ => Some (I32, dst)
-  | LLInt64 _ dst _ => Some (I64, dst)
+(* Generic typing rules *)
+Module Type Typing.
+  Parameter ptr_ty: ty.
+  Parameter ty_env: func -> type_env.
+End Typing.
 
-  | LLFrame _ dst _ => Some (ptr_ty, dst)
-  | LLGlobal _ dst _ => Some (ptr_ty, dst)
+(* LLIR typing rules *)
+Module Target_Typing (ARCH: ArchTy) <: Typing.
+  Include ARCH.
 
-  | LLLd dst _ _ => Some dst
-  | LLUndef dst _ => Some dst
-  | LLUnop dst _ _ _ => Some dst
-  | LLBinop dst _ _ _ _ => Some dst
+  (* Returns the register defined by an instruction and its type. *)
+  Definition get_inst_def (i: inst): option (ty * reg) :=
+    match i with
+    | LLInvoke dst _ _ _ _ => dst
 
-  | LLSt _ _ _ => None
-  | LLRet _ => None
-  | LLJcc _ _ _ => None
-  | LLJmp _ => None
-  end.
+    | LLArg dst _ _ => Some dst
+    | LLInt8 dst _ _ => Some (TInt I8, dst)
+    | LLInt16 dst _ _ => Some (TInt I16, dst)
+    | LLInt32 dst _ _ => Some (TInt I32, dst)
+    | LLInt64 dst _ _ => Some (TInt I64, dst)
 
-Definition ty_env_inst (insts: inst_map): type_env :=
-  PTrie.fold
-    (fun env _ i => 
-      match get_inst_def i with
-      | Some (ty, dst) => PTrie.set env dst ty
-      | None => env
-      end)
-    insts PTrie.empty.
+    | LLFrame _ dst _ => Some (ARCH.ptr_ty, dst)
+    | LLGlobal _ dst _ => Some (ARCH.ptr_ty, dst)
 
-Definition ty_env_phi (phis: phi_map): type_env :=
-  PTrie.fold
-    (fun env _ block =>
-      List.fold_left
-        (fun env p =>
-          match p with
-          | LLPhi (ty, dst) _ => PTrie.set env dst ty
-          end)
-        block env)
-    phis PTrie.empty.
+    | LLLd dst _ _ => Some dst
+    | LLUndef dst _ => Some dst
+    | LLUnop dst _ _ _ => Some dst
+    | LLBinop dst _ _ _ _ => Some dst
 
-Definition ty_env (f: func): type_env :=
-  PTrie.union (ty_env_inst f.(fn_insts)) (ty_env_phi f.(fn_phis)).
+    | LLSt _ _ _ => None
+    | LLRet _ => None
+    | LLJcc _ _ _ => None
+    | LLJmp _ => None
+    end.
 
-Definition well_typed_reg (env: type_env) (r: reg) (ty: ty) :=
-  env ! r = Some ty.
+  (* Type environment from instructions. *)
+  Definition ty_env_inst (insts: inst_map): type_env :=
+    PTrie.fold
+      (fun env _ i =>
+        match get_inst_def i with
+        | Some (ty, dst) => PTrie.set env dst ty
+        | None => env
+        end)
+      insts PTrie.empty.
 
-(*
-Inductive well_typed_inst: type_env -> inst -> Prop := .
-  | typed_jmp:
+  (* Type environment from phis. *)
+  Definition ty_env_phi (phis: phi_map): type_env :=
+    PTrie.fold
+      (fun env _ block =>
+        List.fold_left
+          (fun env p =>
+            match p with
+            | LLPhi (ty, dst) _ => PTrie.set env dst ty
+            end)
+          block env)
+      phis PTrie.empty.
 
-  | LLInvoke dst _ _ _ _ => dst
+  (* Type environment for all registers. *)
+  Definition ty_env (f: func): type_env :=
+    PTrie.union (ty_env_inst f.(fn_insts)) (ty_env_phi f.(fn_phis)).
 
-  | LLArg dst _ _ => Some dst
-  | LLInt8 dst _ _ => Some (I8, dst)
-  | LLInt16 _ dst _ => Some (I16, dst)
-  | LLInt32 _ dst _ => Some (I32, dst)
-  | LLInt64 _ dst _ => Some (I64, dst)
+  (* Holds if the evironment has the correct type for a reg. *)
+  Definition well_typed_reg (env: type_env) (r: reg) (t: ty) :=
+    env ! r = Some t.
 
-  | LLFrame _ dst _ => Some (ptr_ty, dst)
-  | LLGlobal _ dst _ => Some (ptr_ty, dst)
+  (* Typing rules for binary instructions. *)
+  Inductive well_typed_binop: binop -> ty -> ty -> ty -> Prop :=
+    | type_bin_cmp:
+      forall (t: ty) (dt: ty),
+        well_typed_binop LLCmp t t dt
+    | type_bin_add:
+      forall (t: ty),
+        well_typed_binop LLAdd t t t
+    .
 
-  | LLLd dst _ _ => Some dst
-  | LLUndef dst _ => Some dst
-  | LLUnop dst _ _ _ => Some dst
-  | LLBinop dst _ _ _ _ => Some dst
+  (* Typing rules for unary instructions. *)
+  Inductive well_typed_unop: unop -> ty -> ty -> Prop :=
+    .
 
-  | LLSt _ _ _ => None
-  | LLRet _ => None
-  | LLJcc _ _ _ => None
-  | LLJmp _ => None
-  *)
-Definition well_typed_insts (env: type_env) (insts: inst_map) := 
-  False.
+  (* Typing rules for instructions. *)
+  Inductive well_typed_inst: type_env -> inst -> Prop :=
+    | type_jmp:
+      forall (env: type_env) (target: node),
+        well_typed_inst env (LLJmp target)
+    | type_jcc:
+      forall (env: type_env) (cond: reg) (bt: node) (bf: node) (i: ty_int)
+        (COND_TY: well_typed_reg env cond (TInt i)),
+        well_typed_inst env (LLJcc cond bt bf)
+    | type_ret:
+      forall (env: type_env) (ret: reg) (t: ty)
+        (RET_TY: well_typed_reg env ret t),
+        well_typed_inst env (LLRet (Some ret))
+    | type_ret_void:
+      forall (env: type_env),
+        well_typed_inst env (LLRet None)
+    | type_st:
+      forall (env: type_env) (next: node) (addr: reg) (val: reg) (t: ty)
+        (ADDR_TY: well_typed_reg env addr ARCH.ptr_ty)
+        (VAL_TY: well_typed_reg env val t),
+        well_typed_inst env (LLSt next addr val)
+    | type_undef:
+      forall (env: type_env) (next: node) (dst: reg) (t: ty),
+        well_typed_inst env (LLUndef (t, dst) next)
+    | type_ld:
+      forall (env: type_env) (next: node) (dst: reg) (t: ty) (addr: reg)
+        (ADDR_TY: well_typed_reg env addr ARCH.ptr_ty)
+        (DST_TY: well_typed_reg env dst t),
+        well_typed_inst env (LLLd (t, dst) next addr)
+    | type_frame:
+      forall (env: type_env) (dst:reg) (next: node) (object: positive)
+        (DST_TY: well_typed_reg env dst ARCH.ptr_ty),
+        well_typed_inst env (LLFrame dst next object)
+    | type_global:
+      forall (env: type_env) (dst: reg) (next: node) (object: positive)
+        (DST_TY: well_typed_reg env dst ARCH.ptr_ty),
+        well_typed_inst env (LLGlobal dst next object)
+    | type_int8:
+      forall (env: type_env) (dst: reg) (next: node) (val: INT8.t)
+        (DST_TY: well_typed_reg env dst (TInt I8)),
+        well_typed_inst env (LLInt8 dst next val)
+    | type_int16:
+      forall (env: type_env) (dst: reg) (next: node) (val: INT16.t)
+        (DST_TY: well_typed_reg env dst (TInt I16)),
+        well_typed_inst env (LLInt16 dst next val)
+    | type_int32:
+      forall (env: type_env) (dst: reg) (next: node) (val: INT32.t)
+        (DST_TY: well_typed_reg env dst (TInt I32)),
+        well_typed_inst env (LLInt32 dst next val)
+    | type_int64:
+      forall (env: type_env) (dst: reg) (next: node) (val: INT64.t)
+        (DST_TY: well_typed_reg env dst (TInt I64)),
+        well_typed_inst env (LLInt64 dst next val)
+    | type_arg:
+      forall (env: type_env) (t: ty) (dst: reg) (next: node) (idx: nat)
+        (DST_TY: well_typed_reg env dst t),
+        well_typed_inst env (LLArg (t, dst) next idx)
+    | type_binop:
+      forall (env: type_env) (op: binop) (next: node)
+        (l: reg) (tl: ty) (r: reg) (tr: ty) (dst: reg) (t: ty)
+        (LHS_TY: well_typed_reg env l tl)
+        (RHS_TY: well_typed_reg env r tr)
+        (DST_TY: well_typed_reg env dst t)
+        (OP: well_typed_binop op tl tr t),
+        well_typed_inst env (LLBinop (t, dst) next op l r)
+    | type_unop:
+      forall (env: type_env) (op: unop) (next: node)
+        (arg: reg) (argt: ty) (dst: reg) (t: ty)
+        (ARG_TY: well_typed_reg env arg argt)
+        (OP: well_typed_unop op argt t),
+        well_typed_inst env (LLUnop (t, dst) next op arg)
+    | type_invoke_void:
+      forall (env: type_env) (next: node)
+        (dst: reg) (t: ty)
+        (callee: reg) (args: list reg) (exn: option node)
+        (CALLEE_TY: well_typed_reg env callee ARCH.ptr_ty),
+        well_typed_inst env (LLInvoke (Some (t, dst)) next callee args exn)
+    .
 
-Inductive well_typed_phi: type_env -> phi -> Prop :=
-  | typed_phi:
-    forall (env: type_env) (p: phi),
-      well_typed_phi env p
-  .
+  Definition well_typed_insts (env: type_env) (insts: inst_map) :=
+    forall (n: node) (i: inst),
+      Some i = insts ! n -> well_typed_inst env i.
 
-Definition well_typed_phis (env: type_env) (phis: phi_map) :=
-  False.
+  Inductive well_typed_phi: type_env -> phi -> Prop :=
+    | typed_phi:
+      forall (env: type_env) (dst: reg) (t: ty) (ins: list (node * reg))
+        (INS: forall (n: node) (r: reg), In (n, r) ins -> well_typed_reg env r t),
+        well_typed_phi env (LLPhi (t, dst) ins)
+    .
 
-Definition well_typed (f: func) :=
-  well_typed_insts (ty_env f) f.(fn_insts)
-  /\
-  well_typed_phis (ty_env f) f.(fn_phis).
+  Definition well_typed_phis (env: type_env) (phis: phi_map) :=
+    forall (n: node) (block: list phi) (p: phi),
+      Some block = phis ! n ->
+      In p block ->
+      well_typed_phi env p.
 
+  Definition well_typed (f: func) :=
+    well_typed_insts (ty_env f) f.(fn_insts)
+    /\
+    well_typed_phis (ty_env f) f.(fn_phis).
+End Target_Typing.
+
+Module X86_Typing := Target_Typing (X86_ArchTy).
